\documentclass{report}
\usepackage{xcolor}
\usepackage{verbatim}
\usepackage[T1]{fontenc}
\usepackage{hyperref}
\newcommand{\code}[1]{\texttt{#1}}
\newcommand{\R}{R}
\newcommand{\pkg}[1]{#1}
\newcommand{\CRANpkg}[1]{\pkg{#1}}%
\newcommand{\BIOpkg}[1]{\pkg{#1}}
\usepackage{amsmath,amssymb,array}
\usepackage{booktabs}
\usepackage{multirow}
\usepackage{amsthm}
  
\theoremstyle{plain}
\newtheorem{thm}{Theorem}[section]
\newtheorem{lemma}[thm]{Lemma}
 
\theoremstyle{remark}
\newtheorem{remark}[thm]{Remark}
 
\newenvironment{algorithmJP} 
{\def\block{\phantom{a}\hspace{10pt}}\setlength{\parindent}{0pt} \par \vspace{\baselineskip}\hrule% 
\smallskip \ttfamily %This big fun below is to allow the typewriter font to stretch spaces between words a bit.
\fontdimen2\font=0.4em% interword space
\fontdimen3\font=0.2em% interword stretch
\fontdimen7\font=0.1em% extra space
\hyphenchar\font=`\-% to allow hyphenation
}
{\smallskip \hrule \vspace{\baselineskip}\par}
 
\newcommand\rr{\mathcal{R}}
\newcommand\er{\mathbb{R}}
\newcommand\ee{\mathbb{E}}
\newcommand\prob{\mathbb{P}}
\newcommand\X{\mathbb{X}}
\newcommand\en{\mathcal{N}}
\newcommand\I{\mathbf{1}}
 
\newcommand\cvar{\textrm{CVaR}}
\newcommand\lsad{\textrm{LSAD}} 
\newcommand\diag{\mathop{\rm diag}}
\newcommand\varr{\textrm{VaR}}
 
\usepackage{algorithm2e}
\begin{document}
\nopagecolor
 \rmfamily\normalsize
 \begin{algorithmJP} 
 Set  $\nu =0$ and $K_1 = \mathcal{M}$. \\
 Put $cmat = (c+ (q^-)^T{\bar A}, 1)$, $Amat = NULL$, $bmat = NULL$ \\
 
 repeat \\
  \block Put $\nu = \nu+1$\\
  \block Compute $\eta_\nu = \sum_{n\in K_\nu}    p_n (q^+ + q^-)^T A(\omega_n)$ and $\zeta_\nu = \sum_{n\in K_\nu}  p_n (q^+ + q^-)^Tb(\omega_n)$\\
  \block Put $Amat = rbind(Amat, (-\eta_\nu, \zeta_\nu, -1))$, $bmat = c(bmat,0)$\\
  \block Solve the linear problem $\min_{(x,w)} cmat^T*(x,w)$ with the constraints\\
  \block  $Amat * (x,w)^T \le bmat^T$   and denote its solution by $(x^*, w^*)$. \\
  \block Put 
 \begin{align*}
  &K^* = \left\{n\in \mathcal{M}\colon \left(q^+ + q^-\right)^T\left(b\left(\omega_n\right) - A\left(\omega_n\right)x^*\right) \ge 0\right\}, \\
  &w_+^* = \sum_{n\in K^*} p_n \left(q^+ + q^-\right)^T\left(b\left(\omega_n\right) - A\left(\omega_n\right)x^*\right), \quad \hat w^* =  \zeta_\nu - \eta_\nu x^*.
  \end{align*}
 \block Set $K_{\nu +1} = K^*$\\
 \block  Compute
 \[
  \underline{F} = c^Tx^* + \left(q^-\right)^T{\bar A} x^* +  w_+^*, \quad \overline{F} = c^Tx^* +  \left(q^-\right)^T{\bar A} x^* +  \hat w^*. 
 \]
 \block \\
 while $(\overline{F} - \underline{F}) > \varepsilon$\\[2pt]
 
 Output: $x^*$
 \end{algorithmJP}
\end{document}
